Dead code elimination for calls to known runtime functions
- Remove the call if the result is unused
- Take into account that the call does not change the memory.

backend/Deadcode.v
@@ -125,7 +125,7 @@ Function transfer_builtin (app: VA.t) (ef: external_function)
       transfer_builtin_args (kill_builtin_res res ne, nmem_all) args
   end.
 
-Definition transfer (f: function) (approx: PMap.t VA.t)
+Definition transfer (f: function) (dm: defmap) (approx: PMap.t VA.t)
                     (pc: node) (after: NA.t) : NA.t :=
   let (ne, nm) := after in
   match f.(fn_code)!pc with
@@ -151,7 +151,15 @@ Definition transfer (f: function) (approx: PMap.t VA.t)
             nmem_remove nm p (size_chunk chunk))
       else after
   | Some(Icall sig ros args res s) =>
-      (add_needs_all args (add_ros_need_all ros (kill res ne)), nmem_all)
+      match is_known_runtime_function dm ros with
+      | None =>
+          (add_needs_all args (add_ros_need_all ros (kill res ne)), nmem_all)
+      | Some bf =>
+        let nres := nreg ne res in
+        if is_dead nres
+        then after
+        else (add_needs_all args (add_ros_need_all ros (kill res ne)), nm)
+      end
   | Some(Itailcall sig ros args) =>
       (add_needs_all args (add_ros_need_all ros NE.bot),
        nmem_dead_stack f.(fn_stacksize))
@@ -168,13 +176,13 @@ Definition transfer (f: function) (approx: PMap.t VA.t)
 
 Module DS := Backward_Dataflow_Solver(NA)(NodeSetBackward).
 
-Definition analyze (approx: PMap.t VA.t) (f: function): option (PMap.t NA.t) :=
+Definition analyze (f: function) (dm: defmap) (approx: PMap.t VA.t): option (PMap.t NA.t) :=
   DS.fixpoint f.(fn_code) successors_instr
-              (transfer f approx).
+              (transfer f dm approx).
 
 (** * Part 2: the code transformation *)
 
-Definition transf_instr (approx: PMap.t VA.t) (an: PMap.t NA.t)
+Definition transf_instr (dm: defmap) (approx: PMap.t VA.t) (an: PMap.t NA.t)
                         (pc: node) (instr: instruction) :=
   match instr with
   | Iop op args res s =>
@@ -203,6 +211,14 @@ Definition transf_instr (approx: PMap.t VA.t) (an: PMap.t NA.t)
       if nmem_contains (snd an!!pc) p (size_chunk chunk)
       then instr
       else Inop s
+  | Icall sig ros args res s =>
+      match is_known_runtime_function dm ros with
+      | None =>
+          instr
+      | Some bf =>
+          let nres := nreg (fst an!!pc) res in
+          if is_dead nres then Inop s else instr
+      end
   | Ibuiltin (EF_memcpy sz al) (dst :: src :: nil) res s =>
       if nmem_contains (snd an!!pc) (aaddr_arg approx!!pc dst) sz
       then instr
@@ -218,22 +234,22 @@ Definition transf_instr (approx: PMap.t VA.t) (an: PMap.t NA.t)
       instr
   end.
 
-Definition transf_function (rm: romem) (f: function) : res function :=
+Definition transf_function (dm: defmap) (rm: romem) (f: function) : res function :=
   let approx := ValueAnalysis.analyze rm f in
-  match analyze approx f with
+  match analyze f dm approx with
   | Some an =>
       OK {| fn_sig := f.(fn_sig);
             fn_params := f.(fn_params);
             fn_stacksize := f.(fn_stacksize);
-            fn_code := PTree.map (transf_instr approx an) f.(fn_code);
+            fn_code := PTree.map (transf_instr dm approx an) f.(fn_code);
             fn_entrypoint := f.(fn_entrypoint) |}
   | None =>
       Error (msg "Neededness analysis failed")
   end.
 
-Definition transf_fundef (rm: romem) (fd: fundef) : res fundef :=
-  AST.transf_partial_fundef (transf_function rm) fd.
+Definition transf_fundef (dm: defmap) (rm: romem) (fd: fundef) : res fundef :=
+  AST.transf_partial_fundef (transf_function dm rm) fd.
 
 Definition transf_program (p: program) : res program :=
-  transform_partial_program (transf_fundef (romem_for p)) p.
+  transform_partial_program (transf_fundef (prog_defmap p) (romem_for p)) p.
 
